Primes.v
@@ -1,0 +1,107 @@
+(** * Prime numbers over [nat]
+
+    Defines primality, a computable smallest-factor function via trial
+    division, decidability of primality, and Euclid's lemma (derived
+    from Bézout's identity via [Nat.gauss]). *)
+
+From Stdlib Require Import Arith Lia PeanoNat.
+
+Definition prime (p : nat) : Prop :=
+  2 <= p /\ forall d, Nat.divide d p -> d = 1 \/ d = p.
+
+(** ** Smallest factor *)
+
+(** Trial division from [k] up to [n], with structural recursion on [fuel].
+    When fuel runs out we return [n] itself (which always self-divides). *)
+Fixpoint sdf (n k fuel : nat) : nat :=
+  match fuel with
+  | 0 => n
+  | S f => if Nat.eq_dec (n mod k) 0 then k else sdf n (S k) f
+  end.
+
+Definition smallest_factor (n : nat) := sdf n 2 (n - 2).
+
+Lemma sdf_spec : forall fuel n k,
+  2 <= k -> k <= n -> 2 <= n -> n <= k + fuel ->
+  let d := sdf n k fuel in
+  k <= d /\ d <= n /\ n mod d = 0 /\
+  forall j, k <= j -> j < d -> n mod j <> 0.
+Proof.
+  induction fuel as [| f IH]; intros n k Hk Hkn Hn Hb; simpl.
+  - repeat split; [lia | lia | apply Nat.Div0.mod_same | intros; lia].
+  - destruct (Nat.eq_dec (n mod k) 0) as [e | ne].
+    + repeat split; [lia | lia | exact e | intros; lia].
+    + destruct (Nat.eq_dec k n) as [-> | Hkn'].
+      * exfalso. exact (ne (Nat.Div0.mod_same n)).
+      * destruct (IH n (S k) ltac:(lia) ltac:(lia) ltac:(lia) ltac:(lia))
+          as [H1 [H2 [H3 H4]]].
+        repeat split; [lia | lia | exact H3 |].
+        intros j Hj1 Hj2.
+        destruct (Nat.eq_dec j k) as [-> | Hjk]; [exact ne | apply H4; lia].
+Qed.
+
+Lemma smallest_factor_spec : forall n, 2 <= n ->
+  2 <= smallest_factor n /\ smallest_factor n <= n /\
+  Nat.divide (smallest_factor n) n /\
+  forall j, 2 <= j -> j < smallest_factor n -> ~ Nat.divide j n.
+Proof.
+  intros n Hn. unfold smallest_factor.
+  destruct (sdf_spec (n-2) n 2 ltac:(lia) ltac:(lia) ltac:(lia) ltac:(lia))
+    as [H1 [H2 [H3 H4]]].
+  repeat split; [lia | lia | |].
+  - apply Nat.Lcm0.mod_divide. exact H3.
+  - intros j Hj1 Hj2 [q Hq].
+    exact (H4 j ltac:(lia) Hj2 ltac:(rewrite Hq; apply Nat.Div0.mod_mul)).
+Qed.
+
+Lemma smallest_factor_prime : forall n, 2 <= n -> prime (smallest_factor n).
+Proof.
+  intros n Hn.
+  destruct (smallest_factor_spec n Hn) as [Hsf2 [Hsfn [Hdiv Hmin]]].
+  split; [lia |].
+  intros d Hd_div.
+  destruct (Nat.eq_dec d 0) as [-> | Hd0].
+  { destruct Hd_div as [q Hq]. lia. }
+  destruct (Nat.eq_dec d 1) as [-> | Hd1]; [now left |].
+  right.
+  assert (Hd2 : 2 <= d) by (destruct d; [lia |]; destruct d; lia).
+  assert (Hdn : Nat.divide d n) by (eapply Nat.divide_trans; eassumption).
+  destruct (lt_dec d (smallest_factor n)) as [Hlt | Hge].
+  - exfalso. exact (Hmin d Hd2 Hlt Hdn).
+  - destruct Hd_div as [q Hq]. destruct q; lia.
+Qed.
+
+(** ** Decidability *)
+
+Lemma prime_dec : forall n, {prime n} + {~ prime n}.
+Proof.
+  intro n.
+  destruct (le_dec 2 n) as [Hn | Hn].
+  2: { right; intros [H _]; lia. }
+  destruct (Nat.eq_dec (smallest_factor n) n) as [Heq | Hne].
+  - left. rewrite <- Heq. apply smallest_factor_prime. lia.
+  - right. intro Hp.
+    destruct (smallest_factor_spec n Hn) as [Hsf2 [_ [Hdiv _]]].
+    destruct Hp as [_ Hirr]. destruct (Hirr _ Hdiv); lia.
+Qed.
+
+(** ** Euclid's lemma
+
+    Derived from Bézout's identity via [Nat.gauss]: if [p] is prime
+    and [gcd(p, a) = 1] then [p | ab] implies [p | b]. *)
+
+Lemma prime_divides_mul :
+  forall p a b, prime p -> Nat.divide p (a * b) ->
+    Nat.divide p a \/ Nat.divide p b.
+Proof.
+  intros p a b [_ Hirr] Hdiv.
+  destruct (Hirr (Nat.gcd p a) (Nat.gcd_divide_l p a)) as [Hco | Hgp].
+  - right. exact (Nat.gauss p a b Hdiv Hco).
+  - left. rewrite <- Hgp. apply Nat.gcd_divide_r.
+Qed.
+
+Lemma prime_divides_prime :
+  forall p q, prime p -> prime q -> Nat.divide p q -> p = q.
+Proof.
+  intros p q [Hp _] [_ Hirr] Hdiv. destruct (Hirr p Hdiv); lia.
+Qed.
